projectVampire/dafny/test.dfy
@@ -1,0 +1,14 @@
+
+
+class x {
+
+    method c()
+    modifies this 
+    {
+        var a : array<int> := new int[4];
+        var b : array<int> := new int[4];
+        var c : array<int> := new int[4];
+        var s: seq<array<int>> := null;
+        // print(a.Length);
+    }
+}
